theories/Init/LargeElim.v
@@ -4,7 +4,7 @@ Require Import Logic.
 
 Set Universe Polymorphism.
 
-Class LargeElimSort@{s;l|Type~>s} : Type@{l+2} :=
+Class LargeElimSort@{s;l} : Type@{l+2} :=
 { Univ : 𝒰@{s;l+1} ;
   code : 𝒰@{s;l} -> Univ ;
   El : Univ -> 𝒰@{s;l} ;
@@ -13,10 +13,10 @@ Class LargeElimSort@{s;l|Type~>s} : Type@{l+2} :=
 Instance TypeLargeElimSort@{l} : LargeElimSort@{Type;l} := {
     Univ := Type@{l} ; code := fun A => A ; El := fun A => A ; El_code := fun A => eq_refl}.
 
-Definition lift_El@{s;l |Type~>s} {H:LargeElimSort@{s;l}} (A:𝒰@{s;l}) : A -> H.(El) (H.(code) A) :=
+Definition lift_El {H:LargeElimSort} (A:𝒰) : A -> H.(El) (H.(code) A) :=
   fun a => eq_poly _ (fun X => X) a _ (eq_sym (H.(El_code) A)).
 
-Definition unlift_El@{s;l |Type~>s} {H:LargeElimSort@{s;l}} (A:𝒰@{s;l}) : H.(El) (H.(code) A) -> A :=
+Definition unlift_El {H:LargeElimSort} (A:𝒰) : H.(El) (H.(code) A) -> A :=
   fun a => eq_poly _ (fun X => X) a _ (H.(El_code) _).
 
 (* Example of Large Elimination on natural numbers *)
@@ -34,33 +34,33 @@ Definition nat_ind@{} := nat_poly@{Type Prop; 0}.
 Definition nat_sind@{} := nat_poly@{Type SProp; 0}.
 
 
-Definition P@{s;l |Type~>s} {H:LargeElimSort@{s;l}} (n : nat@{s;}) :=
+Definition P {H:LargeElimSort} (n : nat) :=
   match n return H.(Univ) with
     O => code unit
   | _ => code empty
   end.
 
-Lemma eq_true@{s;l |Type~>s} {H:LargeElimSort@{s;l}} : forall (n:nat), O = n -> H.(El) (P n).
+Lemma eq_true {H:LargeElimSort} : forall (n:nat), O = n -> H.(El) (P n).
 Proof.
   intros b e. destruct e. exact (lift_El _ tt).
 Qed.
 
-Lemma nat_discr_gen@{s;l |Type~>s} {H:LargeElimSort@{s;l}} (n : nat@{s;}) : O = S n -> empty@{s;0_}.
+Lemma nat_discr_gen {H:LargeElimSort} (n : nat) : O = S n -> empty.
 Proof.
   intro e. exact (unlift_El _ (eq_true _ e)).
 Qed.
 
 (* Direct Large Elimination *)
 
-Definition Pred_nat@{s ; | s ~> Type} (n : nat@{s;}) :=
+Definition Pred_nat (n : nat) :=
   match n return Type with | O => unit | _ => empty end.
 
-Lemma eq_true'@{s ; | s ~> Type} : forall (n:nat), O = n -> Pred_nat@{s ; } n.
+Lemma eq_true'@{s ; + |+} : forall (n:nat), O = n -> Pred_nat@{s ; _ _} n.
 Proof.
   intros b e. destruct e. exact tt.
 Qed.
 
-Lemma nat_discr@{s ; | s ~> Type} (n : nat@{s;}) : O = S n -> False.
+Lemma nat_discr@{s;} (n : nat@{s;}) : O = S n -> False.
 Proof.
   intro e. destruct (eq_true' _ e).
 Qed.
